<rdf:RDF
    xmlns:rdf="http://www.w3.org/1999/02/22-rdf-syntax-ns#"
    xmlns:provs="http://arcos.rack/PROV-S#"
    xmlns:AGENTS="http://arcos.rack/AGENTS#"
    xmlns:owl="http://www.w3.org/2002/07/owl#"
    xmlns:sadlimplicitmodel="http://sadl.org/sadlimplicitmodel#"
    xmlns:rdfs="http://www.w3.org/2000/01/rdf-schema#"
    xmlns:sadlbasemodel="http://sadl.org/sadlbasemodel#"
    xmlns:xsd="http://www.w3.org/2001/XMLSchema#"
  xml:base="http://arcos.rack/AGENTS">
  <owl:Ontology rdf:about="">
    <owl:imports rdf:resource="PROV-S"/>
    <owl:imports rdf:resource="http://sadl.org/sadlimplicitmodel"/>
    <owl:imports rdf:resource="http://sadl.org/sadlbasemodel"/>
    <rdfs:comment xml:lang="en">This ontology was created from a SADL file 'AGENTS.sadl' and should not be directly edited.</rdfs:comment>
  </owl:Ontology>
  <owl:Class rdf:ID="SOFTWAREAGENT">
    <rdfs:comment xml:lang="en">A software agent is running software.</rdfs:comment>
    <rdfs:subClassOf rdf:resource="PROV-S#AGENT"/>
  </owl:Class>
  <owl:Class rdf:ID="ORGANIZATION">
    <rdfs:comment xml:lang="en">An organization is a social or legal institution such as a company, society, etc.</rdfs:comment>
    <rdfs:subClassOf rdf:resource="PROV-S#AGENT"/>
  </owl:Class>
  <owl:Class rdf:ID="PERSON">
    <rdfs:comment xml:lang="en">Person agents are people</rdfs:comment>
    <rdfs:subClassOf rdf:resource="PROV-S#AGENT"/>
  </owl:Class>
  <owl:ObjectProperty rdf:ID="employedBy">
    <rdfs:subPropertyOf rdf:resource="PROV-S#actedOnBehalfOf"/>
    <rdfs:comment xml:lang="en">Relates people to the company they were acting on behalf of.</rdfs:comment>
    <rdfs:range rdf:resource="PROV-S#AGENT"/>
    <rdfs:domain rdf:resource="#PERSON"/>
  </owl:ObjectProperty>
  <owl:DatatypeProperty rdf:ID="name">
    <rdfs:comment xml:lang="en">Full name of a person</rdfs:comment>
    <rdfs:domain rdf:resource="#PERSON"/>
    <rdfs:comment xml:lang="en">Full name of an organization</rdfs:comment>
    <rdfs:range rdf:resource="http://www.w3.org/2001/XMLSchema#string"/>
    <rdfs:domain rdf:resource="#ORGANIZATION"/>
  </owl:DatatypeProperty>
  <owl:DatatypeProperty rdf:ID="emailAddress">
    <rdfs:comment xml:lang="en">Email address of person</rdfs:comment>
    <rdfs:range rdf:resource="http://www.w3.org/2001/XMLSchema#string"/>
    <rdfs:domain rdf:resource="#PERSON"/>
  </owl:DatatypeProperty>
</rdf:RDF>
