<rdf:RDF
    xmlns:rdf="http://www.w3.org/1999/02/22-rdf-syntax-ns#"
    xmlns:sadlbasemodel="http://sadl.org/sadlbasemodel"
    xmlns:provs="http://arcos.rack/PROV-S"
    xmlns:CONFIDENCE="http://arcos.rack/CONFIDENCE#"
    xmlns:owl="http://www.w3.org/2002/07/owl#"
    xmlns:sadlimplicitmodel="http://sadl.org/sadlimplicitmodel"
    xmlns:builtinfunctions="http://sadl.org/builtinfunctions"
    xmlns:rdfs="http://www.w3.org/2000/01/rdf-schema#"
    xmlns:xsd="http://www.w3.org/2001/XMLSchema#"
  xml:base="http://arcos.rack/CONFIDENCE">
  <owl:Ontology rdf:about="">
    <owl:imports rdf:resource="PROV-S"/>
    <owl:imports rdf:resource="http://sadl.org/builtinfunctions"/>
    <owl:imports rdf:resource="http://sadl.org/sadlimplicitmodel"/>
    <owl:imports rdf:resource="http://sadl.org/sadlbasemodel"/>
    <rdfs:comment xml:lang="en">This ontology was created from a SADL file 'CONFIDENCE.sadl' and should not be directly edited.</rdfs:comment>
  </owl:Ontology>
  <owl:Class rdf:ID="CONFIDENCE_ASSESSMENT">
    <rdfs:comment xml:lang="en">Superclass for confidence assessments over some other data in the ontology.</rdfs:comment>
    <rdfs:subClassOf rdf:resource="PROV-S#THING"/>
  </owl:Class>
  <owl:Class rdf:ID="ASSESSING_CONFIDENCE">
    <rdfs:comment xml:lang="en">ACTIVITY that establishes a CONFIDENCE_ASSESSMENT</rdfs:comment>
    <rdfs:subClassOf rdf:resource="PROV-S#ACTIVITY"/>
  </owl:Class>
  <owl:Class rdf:ID="BDU_CONFIDENCE_ASSESSMENT">
    <rdfs:comment xml:lang="en">A belief-disbelief-uncertainty confidence assessment, c.f. Subjective Logic</rdfs:comment>
    <rdfs:subClassOf rdf:resource="#CONFIDENCE_ASSESSMENT"/>
  </owl:Class>
  <owl:ObjectProperty rdf:ID="assesses">
    <rdfs:subPropertyOf rdf:resource="PROV-S#wasDerivedFrom"/>
    <rdfs:comment xml:lang="en">ENTITY(s) whose confidence is assessed</rdfs:comment>
    <rdfs:range rdf:resource="PROV-S#ENTITY"/>
    <rdfs:domain rdf:resource="#CONFIDENCE_ASSESSMENT"/>
  </owl:ObjectProperty>
  <owl:ObjectProperty rdf:ID="createBy">
    <rdfs:subPropertyOf rdf:resource="PROV-S#wasGeneratedBy"/>
    <rdfs:comment xml:lang="en">ACTIVITY(s) (e.g. ASSESSING_CONFIDENCE) that created this assessment.</rdfs:comment>
    <rdfs:range rdf:resource="PROV-S#ACTIVITY"/>
    <rdfs:domain rdf:resource="#CONFIDENCE_ASSESSMENT"/>
  </owl:ObjectProperty>
  <owl:ObjectProperty rdf:ID="performedBy">
    <rdfs:subPropertyOf rdf:resource="PROV-S#wasAssociatedWith"/>
    <rdfs:comment xml:lang="en">ENTITY responsible for producing the assessment, could be a person or a tool</rdfs:comment>
    <rdfs:range rdf:resource="PROV-S#AGENT"/>
    <rdfs:domain rdf:resource="#ASSESSING_CONFIDENCE"/>
  </owl:ObjectProperty>
  <owl:DatatypeProperty rdf:ID="belief">
    <rdfs:range rdf:resource="http://www.w3.org/2001/XMLSchema#float"/>
    <rdfs:domain rdf:resource="#CONFIDENCE_ASSESSMENT"/>
  </owl:DatatypeProperty>
  <owl:DatatypeProperty rdf:ID="disbelief">
    <rdfs:range rdf:resource="http://www.w3.org/2001/XMLSchema#float"/>
    <rdfs:domain rdf:resource="#CONFIDENCE_ASSESSMENT"/>
  </owl:DatatypeProperty>
  <owl:DatatypeProperty rdf:ID="uncertainty">
    <rdfs:range rdf:resource="http://www.w3.org/2001/XMLSchema#float"/>
    <rdfs:domain rdf:resource="#CONFIDENCE_ASSESSMENT"/>
  </owl:DatatypeProperty>
</rdf:RDF>
