<rdf:RDF
    xmlns:rdf="http://www.w3.org/1999/02/22-rdf-syntax-ns#"
    xmlns:provs="http://arcos.rack/PROV-S#"
    xmlns:owl="http://www.w3.org/2002/07/owl#"
    xmlns:sadlimplicitmodel="http://sadl.org/sadlimplicitmodel#"
    xmlns:rdfs="http://www.w3.org/2000/01/rdf-schema#"
    xmlns:D="http://arcos.rack/DOCUMENT#"
    xmlns:sadlbasemodel="http://sadl.org/sadlbasemodel#"
    xmlns:xsd="http://www.w3.org/2001/XMLSchema#"
  xml:base="http://arcos.rack/DOCUMENT">
  <owl:Ontology rdf:about="">
    <owl:imports rdf:resource="PROV-S"/>
    <owl:imports rdf:resource="http://sadl.org/sadlimplicitmodel"/>
    <owl:imports rdf:resource="http://sadl.org/sadlbasemodel"/>
    <rdfs:comment xml:lang="en">This ontology was created from a SADL file 'DOCUMENT.sadl' and should not be directly edited.</rdfs:comment>
  </owl:Ontology>
  <owl:Class rdf:ID="REQUEST">
    <rdfs:comment xml:lang="en">A REQUEST initiates a defined course of action or changed to fulfill a need.</rdfs:comment>
    <rdfs:subClassOf rdf:resource="PROV-S#COLLECTION"/>
  </owl:Class>
  <owl:Class rdf:ID="SECTION">
    <rdfs:comment xml:lang="en">A SECTION is generic grouping of ENTITYs with a document</rdfs:comment>
    <rdfs:subClassOf rdf:resource="PROV-S#COLLECTION"/>
  </owl:Class>
  <owl:Class rdf:ID="DESCRIPTION">
    <rdfs:comment xml:lang="en">A DESCRIPTION represents a planned or actual concept, function, design or object.</rdfs:comment>
    <rdfs:subClassOf rdf:resource="PROV-S#COLLECTION"/>
  </owl:Class>
  <owl:Class rdf:ID="REPORT">
    <rdfs:comment xml:lang="en">A REPORT describes the results of activities such as investigations, observations, assessments, or test.</rdfs:comment>
    <rdfs:subClassOf rdf:resource="PROV-S#COLLECTION"/>
  </owl:Class>
  <owl:Class rdf:ID="DOC_STATUS">
    <owl:equivalentClass>
      <owl:Class>
        <owl:oneOf rdf:parseType="Collection">
          <D:DOC_STATUS rdf:ID="In_Development"/>
          <D:DOC_STATUS rdf:ID="Released"/>
          <D:DOC_STATUS rdf:ID="Withdrawn"/>
        </owl:oneOf>
      </owl:Class>
    </owl:equivalentClass>
  </owl:Class>
  <owl:Class rdf:ID="SPECIFICATION">
    <rdfs:comment xml:lang="en">A SPECIFICATION identifies, in a complete, precise, and verifiable manner, the requirements, design, behavior, or other expected characteristics of a system, service or process.</rdfs:comment>
    <rdfs:subClassOf rdf:resource="PROV-S#COLLECTION"/>
  </owl:Class>
  <owl:Class rdf:ID="PLAN">
    <rdfs:comment xml:lang="en">A PLAN presents a systematic course of action for achieving a declared purpose, including when, how, and by whom specified activities are to be performed. </rdfs:comment>
    <rdfs:subClassOf rdf:resource="PROV-S#COLLECTION"/>
  </owl:Class>
  <owl:Class rdf:ID="PROCEDURE">
    <rdfs:comment xml:lang="en">A PROCEDURE presents an ordered series of steps to perform a process, activity, or task</rdfs:comment>
    <rdfs:subClassOf rdf:resource="PROV-S#COLLECTION"/>
  </owl:Class>
  <owl:ObjectProperty rdf:ID="approvalAuthority">
    <rdfs:domain rdf:resource="#SPECIFICATION"/>
    <rdfs:domain rdf:resource="#PROCEDURE"/>
    <rdfs:subPropertyOf rdf:resource="PROV-S#wasGeneratedBy"/>
    <rdfs:comment xml:lang="en">AGENT responsible for approving a document.</rdfs:comment>
    <rdfs:range rdf:resource="PROV-S#AGENT"/>
    <rdfs:domain rdf:resource="#PLAN"/>
  </owl:ObjectProperty>
  <owl:ObjectProperty rdf:ID="originatorOfRequest">
    <rdfs:subPropertyOf rdf:resource="PROV-S#wasGeneratedBy"/>
    <rdfs:range rdf:resource="PROV-S#AGENT"/>
    <rdfs:domain rdf:resource="#REQUEST"/>
  </owl:ObjectProperty>
  <owl:ObjectProperty rdf:ID="references">
    <rdfs:domain rdf:resource="#SPECIFICATION"/>
    <rdfs:domain rdf:resource="#PLAN"/>
    <rdfs:subPropertyOf rdf:resource="PROV-S#wasDerivedFrom"/>
    <rdfs:comment xml:lang="en">Source Materials used in the development of a document.</rdfs:comment>
    <rdfs:range rdf:resource="PROV-S#ENTITY"/>
    <rdfs:domain rdf:resource="#DESCRIPTION"/>
  </owl:ObjectProperty>
  <owl:ObjectProperty rdf:ID="issuingOrganization">
    <rdfs:domain rdf:resource="#SPECIFICATION"/>
    <rdfs:domain rdf:resource="#REPORT"/>
    <rdfs:domain rdf:resource="#PROCEDURE"/>
    <rdfs:domain rdf:resource="#PLAN"/>
    <rdfs:subPropertyOf rdf:resource="PROV-S#wasGeneratedBy"/>
    <rdfs:comment xml:lang="en">AGENT responsible for producing a document.</rdfs:comment>
    <rdfs:range rdf:resource="PROV-S#AGENT"/>
    <rdfs:domain rdf:resource="#DESCRIPTION"/>
  </owl:ObjectProperty>
  <owl:ObjectProperty rdf:ID="status">
    <rdfs:domain rdf:resource="#SPECIFICATION"/>
    <rdfs:domain rdf:resource="#REQUEST"/>
    <rdfs:domain rdf:resource="#REPORT"/>
    <rdfs:domain rdf:resource="#PROCEDURE"/>
    <rdfs:domain rdf:resource="#PLAN"/>
    <rdfs:comment xml:lang="en">Identifies the maturity of the document, In_Development, Released, Withdrawn.</rdfs:comment>
    <rdfs:range rdf:resource="#DOC_STATUS"/>
    <rdfs:domain rdf:resource="#DESCRIPTION"/>
  </owl:ObjectProperty>
  <owl:DatatypeProperty rdf:ID="dateOfInitiation">
    <rdfs:range rdf:resource="http://www.w3.org/2001/XMLSchema#date"/>
    <rdfs:domain rdf:resource="#REQUEST"/>
  </owl:DatatypeProperty>
  <owl:DatatypeProperty rdf:ID="dateOfIssue">
    <rdfs:domain rdf:resource="#SPECIFICATION"/>
    <rdfs:domain rdf:resource="#REPORT"/>
    <rdfs:domain rdf:resource="#PROCEDURE"/>
    <rdfs:domain rdf:resource="#PLAN"/>
    <rdfs:comment xml:lang="en">Release date for the document.</rdfs:comment>
    <rdfs:range rdf:resource="http://www.w3.org/2001/XMLSchema#date"/>
    <rdfs:domain rdf:resource="#DESCRIPTION"/>
  </owl:DatatypeProperty>
  <owl:DatatypeProperty rdf:ID="title">
    <rdfs:range rdf:resource="http://www.w3.org/2001/XMLSchema#string"/>
    <rdfs:domain rdf:resource="#SECTION"/>
  </owl:DatatypeProperty>
</rdf:RDF>
